## W3C Web Annotation vocabulary
## http://www.w3.org/ns/oa
##
## Copyright © 2015-2016 W3C ® (MIT, ERCIM, Keio, Beihang).
## W3C liability, trademark use rules apply.
##
## This Document is licensed under the W3C Software and Document license.
## https://www.w3.org/Consortium/Legal/2015/copyright-software-and-document
##
@prefix : <http://www.w3.org/ns/oa> .
@prefix as: <http://www.w3.org/ns/activitystreams#> .
@prefix dc: <http://purl.org/dc/elements/1.1/> .
@prefix oa: <http://www.w3.org/ns/oa#> .
@prefix cnt: <http://www.w3.org/2011/content#> .
@prefix owl: <http://www.w3.org/2002/07/owl#> .
@prefix rdf: <http://www.w3.org/1999/02/22-rdf-syntax-ns#> .
@prefix xml: <http://www.w3.org/XML/1998/namespace> .
@prefix xsd: <http://www.w3.org/2001/XMLSchema#> .
@prefix foaf: <http://xmlns.com/foaf/0.1/> .
@prefix prov: <http://www.w3.org/ns/prov#> .
@prefix rdfs: <http://www.w3.org/2000/01/rdf-schema#> .
@prefix skos: <http://www.w3.org/2004/02/skos/core#> .
@prefix trig: <http://www.w3.org/2004/03/trix/rdfg-1/> .
@prefix dcterms: <http://purl.org/dc/terms/> .
@prefix dctypes: <http://purl.org/dc/dcmitype/> .
@prefix vann: <http://purl.org/vocab/vann/> .

<http://www.w3.org/ns/oa#> a owl:Ontology ;
	owl:versionIRI <http://www.w3.org/TR/2015/WD-annotation-vocab-20160331/oa.ttl> ; #UPDATEME
	owl:versionInfo "WD-20160331" ; #UPDATEME
	rdfs:seeAlso <http://www.w3.org/TR/annotation-model/>, <http://www.w3.org/TR/annotation-vocab/> ;
	dc:title "W3C Web Annotation vocabulary"@en ;
	rdfs:comment "The Web Annotation vocabulary defines the terms corresponding with the Web Annotation Data Model."@en ;
	dc:creator "Robert Sanderson"@en ;
	dc:creator "Paolo Ciccarese"@it ;
	dc:creator "Benjamin Young"@en ;
	dc:contributor "Herbert Van de Sompel"@vls ;
	dc:contributor "Stian Soiland-Reyes"@en ;
	dc:rights "Copyright © 2015-2016 W3C ® (MIT, ERCIM, Keio, Beihang). W3C liability, trademark use rules apply. This Document is licensed under the W3C Software and Document license."@en ;
	dcterms:license <https://www.w3.org/Consortium/Legal/2015/copyright-software-and-document> ;
	dcterms:publisher <http://www.w3.org/data#W3C> ;
	vann:preferredNamespacePrefix "oa" ;
	vann:preferredNamespaceUri "http://www.w3.org/ns/oa#" ;
  vann:usageNote <http://www.w3.org/TR/annotation-vocab/> ;
	owl:backwardCompatibleWith <http://www.openannotation.org/spec/core/20130208/oa.owl> ;
	owl:priorVersion <http://www.openannotation.org/spec/core/20130208/oa.owl> .

## Web Annotation Vocabulary
# Split into:
# - Classes
# - Object properties
# - Datatype properties

#
# #################################################################
# #
# #    Classes
# #
# #################################################################
#
#
#
# http://www.w3.org/ns/oa#Annotation

oa:Annotation a owl:Class ;
	rdfs:isDefinedBy <http://www.w3.org/ns/oa#> ;
	rdfs:label "Annotation"@en ;
	rdfs:comment """The class for Web Annotations"""@en ;
	rdfs:seeAlso <https://www.w3.org/TR/annotation-model/#web-annotation-principles> ,
	   <https://www.w3.org/TR/2016/WD-annotation-vocab-20160331/#annotation> ;
	rdfs:subClassOf [
		a owl:Restriction ;
		owl:onProperty oa:hasTarget ;
		owl:minCardinality "1"^^xsd:nonNegativeInteger
	] ;
	rdfs:subClassOf [
		a owl:Restriction ;
		owl:onProperty oa:hasBody ;
		owl:minCardinality "0"^^xsd:nonNegativeInteger
	] ;
	rdfs:seeAlso oa:motivatedBy, dcterms:creator, dcterms:created, oa:bodyText, oa:styledBy, dcterms:issued, as:generator .

#
# http://www.w3.org/ns/oa#Choice

oa:Choice a owl:Class ;
	rdfs:subClassOf oa:Choice ;
	rdfs:label "Choice"@en ;
	rdfs:comment """A subClass of `as:OrderedCollection` that conveys to a consuming
application that it should select one of the resources in the `as:items` list
to use, rather than all of them. This is typically used to provide a choice
of resources to render to the user, based on further supplied properties.
If the consuming application cannot determine the user's preference,
then it should use the first in the list."""@en ;
	rdfs:seeAlso <https://www.w3.org/TR/2016/WD-annotation-vocab-20160331/#choice> ;
	rdfs:seeAlso <http://w3c.github.io/web-annotation/model/wd2/#choice-of-bodies-and-targets> ;
	rdfs:subClassOf as:OrderedCollection ;
	rdfs:isDefinedBy <http://www.w3.org/ns/oa#> ;
	rdfs:subClassOf [
		a owl:Restriction ;
		owl:onProperty as:items ;
		owl:minCardinality "1"^^xsd:nonNegativeInteger
	] .

#
#
# http://www.w3.org/ns/oa#Content

oa:Content a owl:Class ;
	rdfs:seeAlso <https://www.w3.org/TR/2016/WD-annotation-vocab-20160331/#content> ;
	rdfs:label "Content"@en ;
	rdfs:comment """The class for resources embedded in the `Annotation` graph, other than
for textual content that is the object of the `hasBody` relationship."""@en ;
	rdfs:isDefinedBy <http://www.w3.org/ns/oa#> ;
	rdfs:subClassOf [
	  a owl:Restriction ;
		owl:onProperty oa:text ;
		owl:qualifiedCardinality "1"^^xsd:nonNegativeInteger ;
		owl:onDataRange xsd:string
	] ;
	rdfs:seeAlso dc:language, dcterms:creator, dcterms:created, dcterms:rights .

#
# http://www.w3.org/ns/oa#CssSelector

oa:CssSelector a owl:Class ;
	rdfs:subClassOf oa:Selector ;
	rdfs:comment """A CssSelector describes a Segment of interest in a representation that conforms to the Document Object Model through the use of the CSS selector specification."""@en ;
	rdfs:isDefinedBy <http://www.w3.org/ns/oa#> ;
	rdfs:seeAlso <https://www.w3.org/TR/2016/WD-annotation-vocab-20160331/#cssselector> ;
	rdfs:label "CssSelector"@en .
#
# http://www.w3.org/ns/oa#CssStyle

oa:CssStyle a owl:Class ;
	rdfs:subClassOf oa:Style ;
	rdfs:seeAlso <https://www.w3.org/TR/2016/WD-annotation-vocab-20160331/#cssstyle> ;
	rdfs:comment """A resource which describes styles for resources participating in the Annotation using CSS."""@en ;
	rdfs:isDefinedBy <http://www.w3.org/ns/oa#> ;
	rdfs:label "CssStyle"@en .
#
# http://www.w3.org/ns/oa#DataPositionSelector

oa:DataPositionSelector a owl:Class ;
	rdfs:subClassOf oa:Selector ;
	rdfs:comment """DataPositionSelector describes a range of data by recording
the start and end positions of the selection in the stream. Position 0
would be immediately before the first byte, position 1 would be immediately
before the second byte, and so on. The start byte is thus included
in the list, but the end byte is not."""@en ;
	rdfs:isDefinedBy <http://www.w3.org/ns/oa#> ;
	rdfs:seeAlso <https://www.w3.org/TR/2016/WD-annotation-vocab-20160331/#datapositionselector> ;
	rdfs:label "DataPositionSelector"@en ;
	rdfs:subClassOf [
	  a owl:Restriction ;
		owl:onProperty oa:start ;
		owl:qualifiedCardinality "1"^^xsd:nonNegativeInteger ;
		owl:onDataRange xsd:nonNegativeInteger ;  # NOTE: this is xsd:integer in HTML
	] ;
	rdfs:subClassOf [
		a owl:Restriction ;
		owl:onProperty oa:end ;
		owl:qualifiedCardinality "1"^^xsd:nonNegativeInteger ;
		owl:onDataRange xsd:integer ; # NOTE: this is xsd:integer in HTML
	] .


#
# http://www.w3.org/ns/oa#FragmentSelector

oa:FragmentSelector a owl:Class ;
	rdfs:subClassOf oa:Selector ;
	rdfs:comment """The FragmentSelector class is used to record the segment of a representation using the URI fragment specification defined by the representation's media type.

This class requires a single data property `rdf:value` - but to remain compatible with OWL this is not expressed in the ontology.
	"""@en ;
	rdfs:seeAlso dcterms:conformsTo, rdf:value ;
	rdfs:isDefinedBy <http://www.w3.org/ns/oa#> ;
	rdfs:seeAlso <https://www.w3.org/TR/2016/WD-annotation-vocab-20160331/#fragmentselector> ;
	rdfs:label "FragmentSelector"@en .
#
# http://www.w3.org/ns/oa#HttpRequestState

oa:HttpRequestState a owl:Class ;
	rdfs:label "HttpRequestState"@en ;

	rdfs:seeAlso <https://www.w3.org/TR/2016/WD-annotation-vocab-20160331/#httprequeststate> ;
	rdfs:subClassOf oa:State ;
	rdfs:subClassOf
	 [ a owl:Restriction ;
		owl:onProperty rdf:value ;
		owl:qualifiedCardinality "1"^^xsd:nonNegativeInteger ;
		owl:onDataRange xsd:string
	] .

oa:HttpRequestState rdfs:comment """The HttpRequestState class is used to record the HTTP request headers that a client SHOULD use to request the correct representation from the resource.

There MUST be exactly 1 rdf:value property per HttpRequestState, containing HTTP request headers as a single, complete string, exactly as they would appear in an HTTP request."""@en ;
	rdfs:isDefinedBy <http://www.w3.org/ns/oa#> ;
	rdfs:seeAlso rdf:value ;
	rdfs:label "HttpRequestState"@en .
#
# http://www.w3.org/ns/oa#Motivation

oa:Motivation a owl:Class ;
	rdfs:subClassOf skos:Concept ;
	rdfs:comment """The Motivation class is used to record the user's intent or motivation for the creation of the Annotation, or the inclusion of the body or target, that it is associated with."""@en ;
	rdfs:seeAlso oa:motivatedBy, <https://www.w3.org/TR/2016/WD-annotation-vocab-20160331/#motivation> ;
	rdfs:isDefinedBy <http://www.w3.org/ns/oa#> ;
	rdfs:label "Motivation"@en .

#
# http://www.w3.org/ns/oa#RangeSelector

oa:RangeSelector a owl:Class ;
	rdfs:comment """A Range Selector can be used to identify the beginning and the end of the selection by using other Selectors. The selection consists of everything from the beginning of the starting selector through to the beginning of the ending selector, but not including it."""@en ;
	rdfs:isDefinedBy <http://www.w3.org/ns/oa#> ;
	rdfs:seeAlso <https://www.w3.org/TR/2016/WD-annotation-vocab-20160331/#rangeselector> ;
	rdfs:label "RangeSelector"@en ;
	rdfs:subClassOf oa:Selector ;
	rdfs:subClassOf [
		a owl:Restriction ;
		owl:onProperty oa:hasStartSelector ;
		owl:qualifiedCardinality "1"^^xsd:nonNegativeInteger
	] ;
	rdfs:subClassOf [
		a owl:Restriction ;
		owl:onProperty oa:hasEndSelector ;
		owl:qualifiedCardinality "1"^^xsd:nonNegativeInteger
	] .

#
# http://www.w3.org/ns/oa#ResourceSelection

oa:ResourceSelection a owl:Class ;
	rdfs:comment """Instances of the ResourceSelection class identify part
(described by an oa:Selector) of another resource (referenced with oa:hasSource),
possibly from a particular representation of a resource (described by an oa:State).
Please note that ResourceSelection is not used directly in the Web Annotation model,
but is provided as a separate class for further application profiles to use,
separate from oa:SpecificResource which has many Annotation specific features.
"""@en ;
	rdfs:isDefinedBy <http://www.w3.org/ns/oa#> ;
	rdfs:seeAlso <https://www.w3.org/TR/2016/WD-annotation-vocab-20160331/#resourceselection> ;
	rdfs:seeAlso oa:hasSelector, oa:hasState ;
	rdfs:label "ResourceSelection"@en ;
	rdfs:subClassOf oa:Selector ;
	rdfs:subClassOf [
		a owl:Restriction ;
		owl:onProperty oa:hasSource ;
		owl:qualifiedCardinality "1"^^xsd:nonNegativeInteger
	] .


#
# http://www.w3.org/ns/oa#Selector

oa:Selector a owl:Class ;
	rdfs:comment """A resource which describes the segment of interest in a representation of
a Source resource, indicated with oa:hasSelector from the Specific Resource.

This class should only be used in further ontologies to derive subclasses.
"""@en ;

	rdfs:isDefinedBy <http://www.w3.org/ns/oa#> ;
	rdfs:seeAlso <https://www.w3.org/TR/2016/WD-annotation-vocab-20160331/#selector> ;
	rdfs:seeAlso oa:FragmentSelector, oa:TextQuoteselector, oa:TextPositionSelector, oa:DataPositionSelector, oa:SvgSelector, oa:hasSelector ;
	rdfs:label "Selector"@en .
#
# http://www.w3.org/ns/oa#SpecificResource

oa:SpecificResource a owl:Class ;
	rdfs:comment """Instances of the SpecificResource class identify part of another resource
(referenced with oa:hasSource), a particular representation of a resource, a resource with
styling hints for renders, or any combination of these, as used within an Annotation."""@en ;
	rdfs:subClassOf oa:ResourceSelection ;
	rdfs:isDefinedBy <http://www.w3.org/ns/oa#> ;
	rdfs:seeAlso <https://www.w3.org/TR/2016/WD-annotation-vocab-20160331/#specificresource> ;
	rdfs:seeAlso oa:hasSource, oa:hasSelector, oa:hasState, oa:hasPurpose, oa:hasScope, oa:styleClass ;
	rdfs:label "SpecificResource"@en .
#
# http://www.w3.org/ns/oa#State

oa:State a owl:Class ;
	rdfs:comment """A State describes the intended state of a resource as applied to the particular Annotation, and thus provides the information needed to retrieve the correct representation of that resource.

This class should only be used in further ontologies to derive subclasses.
	"""@en ;
	rdfs:isDefinedBy <http://www.w3.org/ns/oa#> ;
	rdfs:seeAlso <https://www.w3.org/TR/2016/WD-annotation-vocab-20160331/#state> ;
	rdfs:seeAlso oa:HttpRequestState, oa:TimeState ;
	rdfs:label "State"@en .
#
# http://www.w3.org/ns/oa#Style

oa:Style a owl:Class ;
	rdfs:comment """A Style describes the intended styling of a resource as applied
to the particular Annotation, and thus provides the information ndeed to
ensure that rendering is consistent across implementations.

This class should only be used in further ontologies to derive subclasses. """@en ;
	rdfs:isDefinedBy <http://www.w3.org/ns/oa#> ;
	rdfs:seeAlso <https://www.w3.org/TR/2016/WD-annotation-vocab-20160331/#style> ;
	rdfs:seeAlso oa:styledBy ;
	rdfs:label "Style"@en .
#
# http://www.w3.org/ns/oa#SvgSelector

oa:SvgSelector a owl:Class ;
	rdfs:subClassOf oa:Selector ;
	rdfs:comment """An SvgSelector defines an area through the use of the
Scalable Vector Graphics [SVG] standard. This allows the user to select a non-rectangular
area of the content, such as a circle or polygon by describing the region using SVG.
The SVG may be either embedded within the Annotation or referenced as an External Resource.
"""@en ;
	rdfs:seeAlso oa:text, dc:format ;
	rdfs:isDefinedBy <http://www.w3.org/ns/oa#> ;
	rdfs:seeAlso <https://www.w3.org/TR/2016/WD-annotation-vocab-20160331/#svgselector> ;
	rdfs:label "SvgSelector"@en .
#
# http://www.w3.org/ns/oa#TextPositionSelector

oa:TextPositionSelector a owl:Class ;
	rdfs:subClassOf oa:Selector ;
	rdfs:comment """The TextPositionSelector describes a range of text by recording the start and end
	positions of the selection in the stream. Position 0 would be immediately before the first character,
	position 1 would be immediately before the second character, and so on.
"""@en ;
	rdfs:isDefinedBy <http://www.w3.org/ns/oa#> ;
	rdfs:seeAlso <https://www.w3.org/TR/2016/WD-annotation-vocab-20160331/#textpositionselector> ;
	rdfs:label "TextPositionSelector"@en ;
	rdfs:subClassOf [
	  a owl:Restriction ;
		owl:onProperty oa:start ;
		owl:qualifiedCardinality "1"^^xsd:nonNegativeInteger ;
		owl:onDataRange xsd:nonNegativeInteger ;  # NOTE: this is xsd:integer in HTML
	] ;
	rdfs:subClassOf [
		a owl:Restriction ;
		owl:onProperty oa:end ;
		owl:qualifiedCardinality "1"^^xsd:nonNegativeInteger ;
		owl:onDataRange xsd:integer ; # NOTE: this is xsd:integer in HTML
	] .

#
# http://www.w3.org/ns/oa#TextQuoteSelector

oa:TextQuoteSelector a owl:Class ;
	rdfs:subClassOf oa:Selector ;
	rdfs:comment """The TextQuoteSelector describes a range of text by copying it, and
including some of the text immediately before (a prefix) and after (a suffix) it to
distinguish between multiple copies of the same sequence of characters."""@en ;
	rdfs:isDefinedBy <http://www.w3.org/ns/oa#> ;
	rdfs:label "TextQuoteSelector"@en ;
	rdfs:seeAlso oa:prefix, oa:suffix ;
	rdfs:subClassOf [
		a owl:Restriction ;
		owl:onProperty oa:exact ;
		owl:qualifiedCardinality "1"^^xsd:nonNegativeInteger ;
		owl:onDataRange xsd:string ; # NOTE: this is xsd:integer in HTML
	] .
#
# http://www.w3.org/ns/oa#TextualBody

oa:TextualBody a owl:Class ;
	rdfs:subClassOf oa:Content, dctypes:Text .


oa:TextualBody rdfs:comment """In many situations, the body of the Annotation will be in a text format, and created at the same time as the Annotation and not have a separate IRI. In these cases, the Body's text can be included as part of the Annotation to avoid having to interact with multiple systems.

The Body may also have the features of External Web Resources, including especially the language of the text and the format that it is conveyed in.

There MUST be exactly 1 oa:text property associated with the TextualBody."""@en ;
	rdfs:label "TextualBody"@en .
#
# http://www.w3.org/ns/oa#TimeState

oa:TimeState a owl:Class ;
	rdfs:subClassOf oa:State ;
	rdfs:comment """A resource which describes how to retrieve a representation of the Source resource that is temporally appropriate for the Annotation.

There MUST be at least one of oa:cachedSource or oa:when specified. If there is more than 1, each gives an alternative copy of the representation."""@en ;
	rdfs:isDefinedBy <http://www.w3.org/ns/oa#> ;
	rdfs:label "TimeState"@en .



#
# #################################################################
# #
# #    Object Properties
# #
# #################################################################


#
# http://www.w3.org/ns/oa#cachedSource

oa:cachedSource a owl:ObjectProperty ;
	rdfs:domain oa:TimeState ;
	rdfs:comment """A link to a copy of the Source resource's representation, appropriate for the Annotation.

There MAY be 0 or more cached relationships per TimeState. If there is more than 1, each gives an alternative copy of the representation."""@en ;
	rdfs:isDefinedBy <http://www.w3.org/ns/oa#> ;
	rdfs:label "cachedSource"@en .
#
# http://www.w3.org/ns/oa#canonical

oa:canonical a owl:ObjectProperty , owl:FunctionalProperty ;
	rdfs:comment """The relationship between an Annotation, Body or Target and the IRI that SHOULD be used to track its identity, regardless of where it is made accessible.

If this property is set, then systems MUST NOT change or delete it. Systems SHOULD NOT assign a canonical IRI without prior agreement if one is not present, as the Annotation could already have a canonical IRI elsewhere.

There MAY be exactly 1 canonical IRI for each resource."""@en ;
	rdfs:isDefinedBy <http://www.w3.org/ns/oa#> ;
	rdfs:label "canonical"@en ;
	rdfs:seeAlso oa:via .

#
# http://www.w3.org/ns/oa#hasBody

oa:hasBody a owl:ObjectProperty ;
	rdfs:domain oa:Annotation ;
	rdfs:comment """The relationship between an Annotation and its Body.

There SHOULD be 1 or more body relationships associated with an Annotation but there MAY be 0."""@en ;
	rdfs:isDefinedBy <http://www.w3.org/ns/oa#> ;
	rdfs:label "hasBody"@en .
#
# http://www.w3.org/ns/oa#hasPurpose

oa:hasPurpose a owl:ObjectProperty ;
	rdfs:domain oa:TextualBody ;
	rdfs:comment """The reason for the inclusion of the Textual Body within the Annotation.

There MAY be 0 or more purposes associated with a TextualBody."""@en ;
	rdfs:isDefinedBy <http://www.w3.org/ns/oa#> ;
	rdfs:label "hasPurpose"@en .
#
# http://www.w3.org/ns/oa#hasScope

oa:hasScope a owl:ObjectProperty ;
	rdfs:domain oa:SpecificResource ;
	rdfs:comment """The relationship between a Specific Resource and the resource that provides the scope or context for it in this Annotation.

There MAY be 0 or more hasScope relationships for each Specific Resource."""@en ;
	rdfs:isDefinedBy <http://www.w3.org/ns/oa#> ;
	rdfs:label "hasScope"@en .
#
# http://www.w3.org/ns/oa#hasSelector

oa:hasSelector a owl:ObjectProperty ;
	rdfs:domain oa:SpecificResource ;
	rdfs:range oa:Selector ;
	rdfs:comment """The relationship between a oa:SpecificResource and a oa:Selector.

There MUST be exactly 0 or 1 oa:hasSelector relationship associated with a
Specific Resource.

If multiple Selectors are required, either to express a choice between different optional, equivalent selectors, or a chain of selectors that should all be processed, it is necessary to use oa:Choice, oa:Composite or oa:List as a selector."""@en ;
	rdfs:isDefinedBy <http://www.w3.org/ns/oa#> ;
	rdfs:label "hasSelector"@en .
#
# http://www.w3.org/ns/oa#hasSource

oa:hasSource a owl:ObjectProperty, owl:FunctionalProperty ;
	rdfs:domain oa:ResourceSelection ;
	rdfs:comment """The resource that the ResourceSelection, or its subclass SpecificResource, is refined from, or more specific than. Please note that the domain (oa:ResourceSelection) is not used directly in the Web Annotation model."""@en ;
	rdfs:isDefinedBy <http://www.w3.org/ns/oa#> ;
	rdfs:seeAlso <https://www.w3.org/TR/2016/WD-annotation-vocab-20160331/#hassource> ;
	rdfs:label "hasSource"@en .
#
# http://www.w3.org/ns/oa#hasState

oa:hasState a owl:ObjectProperty ;
	rdfs:domain oa:SpecificResource ;
	rdfs:range oa:State ;
	rdfs:comment """The relationship between a oa:SpecificResource and a oa:State resource.

There MAY be 0 or 1 oa:hasState relationship for each SpecificResource.

If there are multiple State resources that must be associated with the specific resource, then the use of the Multiplicity Constructs oa:Choice, oa:Composite or oa:List is RECOMMENDED."""@en ;
	rdfs:isDefinedBy <http://www.w3.org/ns/oa#> ;
	rdfs:label "hasState"@en .
#
# http://www.w3.org/ns/oa#hasTarget

oa:hasTarget a owl:ObjectProperty ;
	rdfs:domain oa:Annotation ;
	rdfs:comment """The relationship between an Annotation and its Target

There MUST be 1 or more `oa:hasTarget` relationships associated with an Annotation.

### Language and format

If the target is an external resource (identified by its IRI), then it SHOULD have exactly 1 `dc:language` associated with it , but MAY have 0 or more. The value of the `dc:language` property SHOULD be a language code following the [rfc5646] specifiction.

If the target is an external resource (identified by its IRI), then it SHOULD have exactly 1 `dc:format` associated with it, but MAY have 0 or more. The value of the property SHOULD be the media-type of the format, following the [rfc6838] specification.


### Creation Information

As the Target and Body may be created at a different time, and by a different agent, from the one that created the Annotation, creation information can be associated with the Body or Target resources body.

dcterms:creator denotes the the agent responsible for creating the Body or Target. This may be either a human or software agent. There MAY be 1 or more dcterms:creator relationships. Creators SHOULD be described as a foaf:Agent (sub)class and its properties.

dcterms:created denotes the time at which the Body or Target was created. There MAY be exactly 1 `dcterms:created` property, and MUST NOT be more than 1. The datetime MUST be expressed in the xsd:dateTime format, and SHOULD have a timezone specified.

### Classes

It is useful for clients to know the general type of a Web Resource in advance. E.g. if the client cannot render videos, then knowing that the Body is a video will allow it to avoid needlessly downloading a potentially large content stream.

Possible classes for typing a target includes dcmi:Dataset, dcmi:Image, dcmi:Video, dcmi:Sound and dcmi:Text."""@en ;
	rdfs:isDefinedBy <http://www.w3.org/ns/oa#> ;
	rdfs:label "hasTarget"@en ;
	rdfs:seeAlso dctypes:Dataset , dctypes:Image , dctypes:Sound , dctypes:Text , dctypes:Video , dcterms:created , dcterms:creator , oa:SpecificResource , oa:TextualBody .

#
# http://www.w3.org/ns/oa#motivatedBy

oa:motivatedBy a owl:ObjectProperty ;
	rdfs:domain oa:Annotation ;
	rdfs:range oa:Motivation ;
	rdfs:comment """The relationship between an Annotation and a Motivation.

There SHOULD be exactly 1 oa:motivatedBy for each Annotation, and MAY be 0 or more than 1."""@en ;
	rdfs:isDefinedBy <http://www.w3.org/ns/oa#> ;
	rdfs:label "motivatedBy"@en .
#
# http://www.w3.org/ns/oa#refinedBy

oa:refinedBy a owl:ObjectProperty ;
	rdfs:domain oa:State ;
	rdfs:range oa:State ;
	rdfs:comment """The relationship between a broader State and the more specific State that should be applied to the results of the first.
Each State MAY be refinedBy 1 or more other States. If more than 1 is given, then they are considered to be alternatives that will result in the same representation."""@en ;
	rdfs:isDefinedBy <http://www.w3.org/ns/oa#> ;
	rdfs:label "refinedBy"@en .

#
# http://www.w3.org/ns/oa#styledBy

oa:styledBy a owl:ObjectProperty ;
	rdfs:domain oa:Annotation ;
	rdfs:range oa:Style ;
	rdfs:comment """The relationship between a oa:Annotation and a oa:Style.

There MAY be 0 or 1 styledBy relationships for each Annotation.

If there are multiple Style resources that must be associated with the Annotation, then the use of the Multiplicity Constructs oa:Choice, oa:Composite or oa:List is RECOMMENDED."""@en ;
	rdfs:isDefinedBy <http://www.w3.org/ns/oa#> ;
	rdfs:label "styledBy"@en .
#
# http://www.w3.org/ns/oa#via

oa:via a owl:ObjectProperty ;
	rdfs:comment """The relationship between an Annotation, Body or Target and the IRI of where that resource was obtained from by the system that is making it available.

There MAY be 0 or more IRIs provided in via for each resource."""@en ;
	rdfs:isDefinedBy <http://www.w3.org/ns/oa#> ;
	rdfs:label "via"@en ;
	rdfs:seeAlso oa:canonical .
#
#
#
# #################################################################
# #
# #    Data properties
# #
# #################################################################
#
#


#
# http://www.w3.org/ns/oa#bodyText

oa:bodyText a owl:DatatypeProperty , owl:FunctionalProperty ;
	rdfs:domain oa:Annotation ;
  rdfs:domain
		[ a owl:Restriction ;
			owl:onProperty oa:hasBody ;
			owl:maxCardinality "0"^^xsd:nonNegativeInteger ] ;
  rdfs:range xsd:string ;
	rdfs:label "bodyText"@en ;
	rdfs:comment """The string value of the body of the Annotation.

There MAY be exactly 1 oa:bodyText for an Annotation, and the value MUST conform to the requirements below. If the bodyText property is present, then the body relationship MUST NOT also be present.

The simplest type of Body is a plain text string, without additional information or properties. This type of body is useful for the simplest of Annotations only, and is NOT RECOMMENDED for uses where the body may need to be referred to from outside of the Annotation.

There are several restrictions on when this form may be used and how it is to be interpreted.

The string body:

* MUST be a single xsd:string and the data type MUST NOT be expressed in the serialization.
* MUST NOT have a language associated with it.
* MUST be interpreted as if it were the value of the text property of a Textual Body.
* MUST be interpreted as if the Textual Body resource had a format property with the value text/plain.
* MUST be interpreted as if the Textual Body resource had a purpose property with the value of commenting.
* MUST NOT have the value of other properties of the Textual Body inferred from similar properties on the Annotation resource."""@en ;
	rdfs:isDefinedBy <http://www.w3.org/ns/oa#> .
#
# http://www.w3.org/ns/oa#end

oa:end a owl:DatatypeProperty ;
	rdfs:domain oa:Selector ;
	rdfs:range xsd:nonNegativeInteger ; # NOTE: this is xsd:integer in HTML
	rdfs:comment """The end position of the segment of text or bytes. The first character/byte in the full text/stream is position 0. The character/byte indicated at position oa:end is NOT included within the selected segment.

See oa:DataPositionSelector and oa:oa:TextPositionSelector."""@en ;
	rdfs:isDefinedBy <http://www.w3.org/ns/oa#> ;
	rdfs:label "end"@en .
#
# http://www.w3.org/ns/oa#exact

oa:exact a owl:DatatypeProperty ;
	#rdfs:domain oa:TextQuoteSelector ; ## TODO: Why is domain not explicit?
	rdfs:range xsd:string ;
	rdfs:comment """A copy of the text which is being selected, after normalization."""@en ;
	rdfs:seeAlso oa:TextQuoteSelector ;
	rdfs:isDefinedBy <http://www.w3.org/ns/oa#> ;
	rdfs:label "exact"@en .
#
# http://www.w3.org/ns/oa#prefix

oa:prefix a owl:DatatypeProperty ;
	#rdfs:domain oa:TextQuoteSelector ; ## TODO: Why is domain not explicit?
	rdfs:range xsd:string ;
	rdfs:comment """A snippet of text that occurs immediately before the text which is being selected.

See oa:TextQuoteSelector."""@en ;
	rdfs:isDefinedBy <http://www.w3.org/ns/oa#> ;
	rdfs:label "prefix"@en .
#
# http://www.w3.org/ns/oa#sourceDate

oa:sourceDate a owl:DatatypeProperty ;
	rdfs:domain oa:TimeState , _:genid2 .

_:genid2 a owl:Restriction ;
	owl:onProperty oa:sourceDateEnd ;
	owl:maxQualifiedCardinality "0"^^xsd:nonNegativeInteger ;
	owl:onDataRange xsd:dateTime .

oa:sourceDate rdfs:domain _:genid3 .

_:genid3 a owl:Restriction ;
	owl:onProperty oa:sourceDateStart ;
	owl:maxQualifiedCardinality "0"^^xsd:nonNegativeInteger ;
	owl:onDataRange xsd:dateTime .

oa:sourceDate rdfs:range xsd:dateTime ;
	rdfs:comment """The timestamp at which the Source resource should be interpreted for the Annotation.

There MAY be 0 or more oa:sourceDate properties per oa:TimeState. If there is more than 1, each gives an alternative timestamp at which the Source may be interpreted. The timestamp MUST be expressed in the xsd:dateTime format, and SHOULD have a timezone specified. If sourceDate is provided, then sourceDateStart and sourceDateEnd MUST NOT be provided."""@en ;
	rdfs:isDefinedBy <http://www.w3.org/ns/oa#> ;
	rdfs:label "sourceDate"@en .
#
# http://www.w3.org/ns/oa#sourceDateEnd

oa:sourceDateEnd a owl:DatatypeProperty , owl:FunctionalProperty ;
	rdfs:domain oa:TimeState , _:genid4 .

_:genid4 a owl:Restriction ;
	owl:onProperty oa:sourceDateStart ;
	owl:someValuesFrom xsd:dateTime .

oa:sourceDateEnd rdfs:range xsd:dateTime ;
	rdfs:comment """The timestamp that ends the interval over which the Source resource should be interpreted for the Annotation.

There MAY be exactly 1 oa:sourceDateEnd property per TimeState. The timestamp MUST be expressed in the xsd:dateTime format, and SHOULD have a timezone specified. If sourceDateEnd is provided then sourceDateStart MUST also be provided."""@en ;
	rdfs:isDefinedBy <http://www.w3.org/ns/oa#> ;
	rdfs:label "sourceDateEnd"@en .
#
# http://www.w3.org/ns/oa#sourceDateStart

oa:sourceDateStart a owl:DatatypeProperty , owl:FunctionalProperty ;
	rdfs:domain oa:TimeState , _:genid5 .

_:genid5 a owl:Restriction ;
	owl:onProperty oa:sourceDateEnd ;
	owl:someValuesFrom xsd:dateTime .

oa:sourceDateStart rdfs:range xsd:dateTime ;
	rdfs:comment """The timestamp that begins the interval over which the Source resource should be interpreted for the Annotation.

There MAY be exactly 1 oa:sourceDateStart property per TimeState. The timestamp MUST be expressed in the xsd:dateTime format, and SHOULD have a timezone specified. If sourceDateStart is provided then sourceDateEnd MUST also be provided."""@en ;
	rdfs:isDefinedBy <http://www.w3.org/ns/oa#> ;
	rdfs:label "sourceDateStart"@en .
#
# http://www.w3.org/ns/oa#start

oa:start a owl:DatatypeProperty ;
	rdfs:domain oa:Selector ;
	rdfs:range xsd:nonNegativeInteger ; # NOTE: this is xsd:integer in HTML
	rdfs:comment """The starting position of the segment of text or bytes. The first character/byte in the full text/stream is position 0. The character/byte indicated at position oa:start is included within the selected segment.

See oa:DataPositionSelector and oa:TextPositionSelector."""@en ;
	rdfs:isDefinedBy <http://www.w3.org/ns/oa#> ;
	rdfs:label "start"@en .
#
# http://www.w3.org/ns/oa#styleClass

oa:styleClass a owl:DatatypeProperty ;
	rdfs:domain oa:SpecificResource ;
	rdfs:comment """The string name of the class used in the CSS description that should be applied to the Specific Resource.

There MAY be 0 or more styleClass properties on a Specific Resource.

See oa:CssStyle."""@en ;
	rdfs:isDefinedBy <http://www.w3.org/ns/oa#> ;
	rdfs:label "styleClass"@en .
#
# http://www.w3.org/ns/oa#suffix

oa:suffix a owl:DatatypeProperty ;
	#rdfs:domain oa:TextQuoteSelector ; ## TODO: Why is domain not explicit?
	rdfs:comment """The snippet of text that occurs immediately after the text which is being selected.

"""@en ;
	rdfs:seeAlso oa:TextQuoteSelector ;
	rdfs:isDefinedBy <http://www.w3.org/ns/oa#> ;
	rdfs:label "suffix"@en .
#
# http://www.w3.org/ns/oa#text

oa:text a owl:DatatypeProperty , owl:FunctionalProperty ;
	rdfs:domain oa:TextualBody ;
	rdfs:comment """The character sequence of the content of the Textual Body.

There MUST be exactly 1 `oa:text` property associated with the `oa:TextualBody`"""@en ;
	rdfs:isDefinedBy <http://www.w3.org/ns/oa#> ;
	rdfs:label "text"@en .
#
# http://www.w3.org/ns/oa#when

oa:when a owl:DatatypeProperty ;
	rdfs:domain oa:TimeState ;
	rdfs:range xsd:dateTimeStamp ;
	rdfs:isDefinedBy <http://www.w3.org/ns/oa#> , "true"^^xsd:boolean .
#
#
#
# #################################################################
# #
# #    Individuals
# #
# #################################################################
#
#
# http://www.w3.org/ns/oa#

<http://www.w3.org/ns/oa#> a owl:NamedIndividual ;
	dcterms:modified "2016-03-20T16:50:00Z"^^xsd:dateTimeStamp .
#
# http://www.w3.org/ns/oa#bookmarking

oa:bookmarking a owl:NamedIndividual , oa:Motivation ;
	rdfs:comment "The motivation for when the user intends to create a bookmark to the Target or part thereof. For example an Annotation that bookmarks the point in a text where the reader finished reading."@en ;
	rdfs:isDefinedBy <http://www.w3.org/ns/oa#> ;
	skos:inScheme oa:motivationScheme ;
	skos:prefLabel "bookmarking"@en .
#
# http://www.w3.org/ns/oa#classifying

oa:classifying a owl:NamedIndividual , oa:Motivation ;
	rdfs:comment "The motivation for when the user intends to that classify the Target as something. For example to classify an image as a portrait."@en ;
	rdfs:isDefinedBy <http://www.w3.org/ns/oa#> ;
	skos:inScheme oa:motivationScheme ;
	skos:prefLabel "classifying"@en .
#
# http://www.w3.org/ns/oa#commenting

oa:commenting a owl:NamedIndividual , oa:Motivation ;
	rdfs:comment "The motivation for when the user intends to comment about the Target. For example to provide a commentary about a particular PDF document."@en ;
	rdfs:isDefinedBy <http://www.w3.org/ns/oa#> ;
	skos:inScheme oa:motivationScheme ;
	skos:prefLabel "commenting"@en .
#
# http://www.w3.org/ns/oa#describing

oa:describing a owl:NamedIndividual , oa:Motivation ;
	rdfs:comment "The motivation for when the user intends to describe the Target, as opposed to a comment about them. For example describing the above PDF's contents, rather than commenting on their accuracy."@en ;
	rdfs:isDefinedBy <http://www.w3.org/ns/oa#> ;
	skos:inScheme oa:motivationScheme ;
	skos:prefLabel "describing"@en .
#
# http://www.w3.org/ns/oa#editing

oa:editing a owl:NamedIndividual , oa:Motivation ;
	rdfs:comment "The motivation for when the user intends to request a change or edit to the Target resource. For example an Annotation that requests a typo to be corrected."@en ;
	rdfs:isDefinedBy <http://www.w3.org/ns/oa#> ;
	skos:inScheme oa:motivationScheme ;
	skos:prefLabel "editing"@en .
#
# http://www.w3.org/ns/oa#highlighting

oa:highlighting a owl:NamedIndividual , oa:Motivation ;
	rdfs:comment "The motivation for when the user intends to highlight the Target resource or segment of it. For example to draw attention to the selected text that the annotator disagrees with."@en ;
	rdfs:isDefinedBy <http://www.w3.org/ns/oa#> ;
	skos:inScheme oa:motivationScheme ;
	skos:prefLabel "highlighting"@en .
#
# http://www.w3.org/ns/oa#identifying

oa:identifying a owl:NamedIndividual , oa:Motivation ;
	rdfs:comment "The motivation for when the user intends to assign an identity to the Target. For example to associate the IRI that identifies a city with a mention of the city in a web page."@en ;
	rdfs:isDefinedBy <http://www.w3.org/ns/oa#> ;
	skos:inScheme oa:motivationScheme ;
	skos:prefLabel "identifying"@en .
#
# http://www.w3.org/ns/oa#linking

oa:linking a owl:NamedIndividual , oa:Motivation ;
	rdfs:comment "The motivation for when the user intends to link to a resource related to the Target."@en ;
	rdfs:isDefinedBy <http://www.w3.org/ns/oa#> ;
	skos:inScheme oa:motivationScheme ;
	skos:prefLabel "linking"@en .
#
# http://www.w3.org/ns/oa#moderating

oa:moderating a owl:NamedIndividual , oa:Motivation ;
	rdfs:comment "The motivation for when the user intends to assign some value or quality to the Target. For example annotating an Annotation to moderate it up in a trust network or threaded discussion."@en ;
	rdfs:isDefinedBy <http://www.w3.org/ns/oa#> ;
	skos:inScheme oa:motivationScheme ;
	skos:prefLabel "moderating"@en .
#
# http://www.w3.org/ns/oa#motivationScheme

oa:motivationScheme a owl:NamedIndividual , skos:ConceptScheme ;
	rdfs:comment "The concept scheme for Open Annotation Motivations"@en ;
	rdfs:isDefinedBy <http://www.w3.org/ns/oa#> ;
	rdfs:label "motivationScheme"@en .
#
# http://www.w3.org/ns/oa#questioning

oa:questioning a owl:NamedIndividual , oa:Motivation ;
	rdfs:comment "The motivation for when the user intends to ask a question about the Target. For example to ask for assistance with a particular section of text, or question its veracity."@en ;
	rdfs:isDefinedBy <http://www.w3.org/ns/oa#> ;
	skos:inScheme oa:motivationScheme ;
	skos:prefLabel "questioning"@en .
#
# http://www.w3.org/ns/oa#replying

oa:replying a owl:NamedIndividual , oa:Motivation ;
	rdfs:comment "The motivation for when the user intends to reply to a previous statement, either an Annotation or another resource. For example providing the assistance requested in the above."@en ;
	rdfs:isDefinedBy <http://www.w3.org/ns/oa#> ;
	skos:inScheme oa:motivationScheme ;
	skos:prefLabel "replying"@en .
#
# http://www.w3.org/ns/oa#reviewing

oa:reviewing a owl:NamedIndividual , oa:Motivation ;
	rdfs:comment "The motivation for when the user intends to review the Target in some assessing fashion, rather than simply make a comment about it. For example to write a review of a Book."@en ;
	rdfs:isDefinedBy <http://www.w3.org/ns/oa#> ;
	skos:inScheme oa:motivationScheme ;
	skos:prefLabel "reviewing"@en .
#
# http://www.w3.org/ns/oa#tagging

oa:tagging a owl:NamedIndividual , oa:Motivation ;
	rdfs:comment "The motivation for when the user intends to associate a tag with the Target."@en ;
	rdfs:isDefinedBy <http://www.w3.org/ns/oa#> ;
	skos:inScheme oa:motivationScheme ;
	skos:prefLabel "tagging"@en .




## Deprecated properties
# from http://www.openannotation.org/spec/core/20130208/
# To discourage use, these have owl:deprecated "true, and
# no longer have any descriptions or
# upper superclass relations


# http://www.w3.org/ns/oa#annotatedBy
oa:annotatedBy a owl:ObjectProperty ;
	rdfs:isDefinedBy <http://www.w3.org/ns/oa#> ;
	rdfs:seeAlso dcterms:creator ;
	owl:deprecated "true"^^xsd:boolean .
#
# http://www.w3.org/ns/oa#default
oa:default a owl:ObjectProperty ;
	rdfs:subPropertyOf oa:item ;
	rdfs:domain oa:Choice ;
	rdfs:isDefinedBy <http://www.w3.org/ns/oa#> ;
	owl:deprecated "true"^^xsd:boolean .
#
# http://www.w3.org/ns/oa#equivalentTo
oa:equivalentTo a owl:ObjectProperty ;
	rdfs:isDefinedBy <http://www.w3.org/ns/oa#> ;
	rdfs:seeAlso oa:canonical , oa:via ;
	owl:deprecated "true"^^xsd:boolean .
#
#
# http://www.w3.org/ns/oa#item
oa:item a owl:ObjectProperty ;
	rdfs:isDefinedBy <http://www.w3.org/ns/oa#> ;
	rdfs:seeAlso as:items ;
	owl:deprecated "true"^^xsd:boolean .
#
#
# http://www.w3.org/ns/oa#serializedBy
oa:serializedBy a owl:ObjectProperty ;
	rdfs:isDefinedBy <http://www.w3.org/ns/oa#> ;
	rdfs:seeAlso as:generator ;
	owl:deprecated "true"^^xsd:boolean .
#
#
# http://www.w3.org/ns/oa#annotatedAt
oa:annotatedAt a owl:DatatypeProperty ;
	rdfs:isDefinedBy <http://www.w3.org/ns/oa#> ;
	owl:deprecated "true"^^xsd:boolean .
#
#
# http://www.w3.org/ns/oa#serializedAt
oa:serializedAt a owl:DatatypeProperty ;
	rdfs:isDefinedBy <http://www.w3.org/ns/oa#> ;
	owl:deprecated "true"^^xsd:boolean .
#
#
# http://www.w3.org/ns/oa#Composite

oa:Composite a owl:Class ;
	rdfs:isDefinedBy <http://www.w3.org/ns/oa#> ;
	owl:deprecated "true"^^xsd:boolean .
#
#
# http://www.w3.org/ns/oa#List

oa:List a owl:Class ;
	rdfs:subClassOf oa:Composite ;
	rdfs:isDefinedBy <http://www.w3.org/ns/oa#> ;
	owl:deprecated "true"^^xsd:boolean .
#
#
# http://www.w3.org/ns/oa#SemanticTag

oa:SemanticTag a owl:Class ;
	rdfs:subClassOf oa:Tag ;
	rdfs:isDefinedBy <http://www.w3.org/ns/oa#> ;
	owl:deprecated "true"^^xsd:boolean .
#
# http://www.w3.org/ns/oa#Tag
oa:Tag a owl:Class ;
	rdfs:isDefinedBy <http://www.w3.org/ns/oa#> ;
	owl:deprecated "true"^^xsd:boolean .


## Cited properties and Classes
#
# Rather than using owl:imports - which can cause network issues and
# import non-related terms, we cite the relevant properties from other
# vocabularies below.  This includes both properties used
# by the Annotation Vocabulary, e.g. Annotation Streams, and also
# properties used to annotate this ontology itself (dcterms and vann)

# See rdfs:isDefinedBy for their defining vocabulary, and
# rdfs:seeAlso for human-readable help
#
#

# http://purl.org/dc/elements/1.1/creator

dc:creator a owl:AnnotationProperty ;
	rdfs:isDefinedBy <http://purl.org/dc/elements/1.1/> .

# http://purl.org/dc/elements/1.1/contributor

dc:contributor a owl:AnnotationProperty ;
	rdfs:isDefinedBy <http://purl.org/dc/elements/1.1/> .

# http://purl.org/dc/elements/1.1/format

dc:format a owl:AnnotationProperty ;
	rdfs:isDefinedBy <http://purl.org/dc/elements/1.1/> .
#
# http://purl.org/dc/elements/1.1/language

dc:language a owl:AnnotationProperty ;
	rdfs:isDefinedBy <http://purl.org/dc/elements/1.1/> .
#
# http://purl.org/dc/elements/1.1/title

dc:title a owl:AnnotationProperty ;
  rdfs:isDefinedBy <http://purl.org/dc/elements/1.1/> .


## Citations from http://purl.org/dc/terms/

#
# http://purl.org/dc/terms/creator

dcterms:creator a owl:ObjectProperty ;
	rdfs:isDefinedBy <http://purl.org/dc/terms/> ;
	rdfs:seeAlso <http://dublincore.org/documents/dcmi-terms/#terms-creator> .
#
# http://purl.org/dc/terms/license

dcterms:license a owl:ObjectProperty ;
  rdfs:isDefinedBy <http://purl.org/dc/terms/> ;
	rdfs:seeAlso <http://dublincore.org/documents/dcmi-terms/#terms-license> .
#
# http://purl.org/dc/terms/publisher
dcterms:publisher a owl:ObjectProperty ;
  rdfs:isDefinedBy <http://purl.org/dc/terms/> ;
	rdfs:seeAlso <http://dublincore.org/documents/dcmi-terms/#terms-publisher> .
#
# http://purl.org/dc/terms/rights
dcterms:rights a owl:ObjectProperty ;
  rdfs:isDefinedBy <http://purl.org/dc/terms/> ;
	rdfs:seeAlso <http://dublincore.org/documents/dcmi-terms/#terms-rights> .

#
# http://purl.org/dc/terms/created

dcterms:created a owl:DatatypeProperty ;
	rdfs:isDefinedBy <http://purl.org/dc/terms/> ;
	rdfs:seeAlso <http://dublincore.org/documents/dcmi-terms/#terms-created> .
#
# http://purl.org/dc/terms/issued

dcterms:issued a owl:DatatypeProperty ;
	rdfs:isDefinedBy <http://purl.org/dc/terms/> ;
	rdfs:seeAlso <http://dublincore.org/documents/dcmi-terms/#terms-issued> .
#
# http://purl.org/dc/terms/modified

dcterms:modified a owl:DatatypeProperty ;
	rdfs:isDefinedBy <http://purl.org/dc/terms/> ;
	rdfs:seeAlso <http://dublincore.org/documents/dcmi-terms/#terms-modified> .


## Citations from http://purl.org/dc/dcmitype/
#

# http://purl.org/dc/dcmitype/Dataset

dctypes:Dataset a owl:Class ;
	rdfs:comment "The class for a resource which encodes data in a defined structure"@en ;
	rdfs:isDefinedBy <http://purl.org/dc/dcmitype/> .
#
# http://purl.org/dc/dcmitype/Image

dctypes:Image a owl:Class ;
	rdfs:comment "The class for image resources, primarily intended to be seen"@en ;
	rdfs:isDefinedBy <http://purl.org/dc/dcmitype/> .
#
# http://purl.org/dc/dcmitype/Sound

dctypes:Sound a owl:Class ;
	rdfs:comment "The class for a resource primarily intended to be heard"@en ;
	rdfs:isDefinedBy <http://purl.org/dc/dcmitype/> .
#
# http://purl.org/dc/dcmitype/Text

dctypes:Text a owl:Class ;
	rdfs:comment "The class for a resource primarily intended to be read"@en ;
	rdfs:isDefinedBy <http://purl.org/dc/dcmitype/> .

# http://purl.org/dc/dcmitype/Video

dctypes:Video a owl:Class ;
	rdfs:comment "The class for video resources, with or without audio"@en ;
	rdfs:isDefinedBy <http://purl.org/dc/dcmitype/> .


## Citations from http://www.w3.org/2004/02/skos/core#

#
# http://www.w3.org/2004/02/skos/core#inScheme
skos:inScheme a owl:AnnotationProperty ;
	rdfs:isDefinedBy <http://www.w3.org/2004/02/skos/core#> ;
	rdfs:seeAlso <https://www.w3.org/TR/skos-reference/#schemes> .
#
# http://www.w3.org/2004/02/skos/core#prefLabel
skos:prefLabel a owl:AnnotationProperty ;
	rdfs:isDefinedBy <http://www.w3.org/2004/02/skos/core#> ;
	rdfs:seeAlso <https://www.w3.org/TR/skos-reference/#labels> .

#
# http://www.w3.org/2004/02/skos/core#Concept

skos:Concept a owl:Class ;
	rdfs:isDefinedBy <http://www.w3.org/2004/02/skos/core#> ;
	rdfs:label "skos:Concept"@en ;
	rdfs:seeAlso <https://www.w3.org/TR/skos-reference/#concepts> .
#
# http://www.w3.org/2004/02/skos/core#ConceptScheme

skos:ConceptScheme a owl:Class ;
	rdfs:isDefinedBy <http://www.w3.org/2004/02/skos/core#> ;
	rdfs:label "skos:ConceptScheme"@en ;
	rdfs:seeAlso <https://www.w3.org/TR/skos-reference/#schemes> .


# Citations from http://xmlns.com/foaf/0.1/

#
# http://xmlns.com/foaf/0.1/Agent

foaf:Agent a owl:Class ;
	rdfs:isDefinedBy <http://xmlns.com/foaf/0.1/> ;
	rdfs:seeAlso <http://xmlns.com/foaf/spec/#term_Agent> .

#
# http://xmlns.com/foaf/0.1/Organization

foaf:Organization a owl:Class ;
	rdfs:subClassOf foaf:Agent ;
	rdfs:isDefinedBy <http://xmlns.com/foaf/0.1/> ;
	rdfs:seeAlso <http://xmlns.com/foaf/spec/#Organization> .
#
# http://xmlns.com/foaf/0.1/Person

foaf:Person a owl:Class ;
	rdfs:subClassOf foaf:Agent ;
	rdfs:isDefinedBy <http://xmlns.com/foaf/0.1/> ;
	rdfs:seeAlso <http://xmlns.com/foaf/spec/#Person> .
#
# http://xmlns.com/foaf/0.1/homepage
foaf:homepage a owl:ObjectProperty ;
	rdfs:isDefinedBy <http://xmlns.com/foaf/0.1/> ;
	rdfs:seeAlso <http://xmlns.com/foaf/spec/#term_homepage> .
#
# http://xmlns.com/foaf/0.1/mbox
foaf:mbox a owl:ObjectProperty , owl:InverseFunctionalProperty ;
	rdfs:domain foaf:Agent ;
	rdfs:isDefinedBy <http://xmlns.com/foaf/0.1/> ;
	rdfs:seeAlso <http://xmlns.com/foaf/spec/#term_mbox> .
#
# http://xmlns.com/foaf/0.1/mbox_sha1sum

foaf:mbox_sha1sum a owl:DatatypeProperty ;
	rdfs:isDefinedBy <http://xmlns.com/foaf/0.1/> ;
	rdfs:seeAlso <http://xmlns.com/foaf/spec/#term_mbox_sha1sum> .
#
# http://xmlns.com/foaf/0.1/name

foaf:name a owl:DatatypeProperty ;
	rdfs:isDefinedBy <http://xmlns.com/foaf/0.1/> ;
  rdfs:seeAlso <http://xmlns.com/foaf/spec/#term_name> .
#
# http://xmlns.com/foaf/0.1/nick

foaf:nick a owl:ObjectProperty ;
	rdfs:domain foaf:Person ;
	rdfs:isDefinedBy <http://xmlns.com/foaf/0.1/> ;
	rdfs:seeAlso <http://xmlns.com/foaf/spec/#term_nick> .





## Citations from
# http://www.w3.org/ns/activitystreams#
#
# As activitystreams is not available as an OWL/RDFS vocabulary,
# but only as HTML/JSON-LD, this includes the label and comment.
#
# Note that the below is NOT a complete representation of
# http://www.w3.org/TR/activitystreams-vocabulary/

# http://www.w3.org/ns/activitystreams#first

as:first a owl:ObjectProperty , owl:FunctionalProperty ;
	rdfs:domain as:CollectionPage ;
	rdfs:range as:CollectionPage ;
	rdfs:comment "In a paged Collection, indicates the furthest preceeding page of items in the collection."@en ;
	rdfs:isDefinedBy <http://www.w3.org/ns/activitystreams> ;
	rdfs:label "first"@en ;
	rdfs:seeAlso as:last , <https://www.w3.org/TR/activitystreams-vocabulary/#dfn-first> .
#
# http://www.w3.org/ns/activitystreams#generator

as:generator a owl:ObjectProperty ;
	rdfs:comment "Identifies the entity (e.g. an application) that generated the object."@en ;
	rdfs:isDefinedBy <http://www.w3.org/ns/activitystreams> ;
	rdfs:label "generator"@en ;
	rdfs:seeAlso <https://www.w3.org/TR/activitystreams-vocabulary/#dfn-generator> .
#
# http://www.w3.org/ns/activitystreams#items

as:items a owl:ObjectProperty ;
	rdfs:domain as:Collection ;
	rdfs:comment """Identifies the items contained in a collection. The items might be ordered or unordered.

The range of this property is rdf:List, but for compatibility with OWL this is
not formally expressed in this ontology.
"""@en ;
	rdfs:isDefinedBy <http://www.w3.org/ns/activitystreams> ;
	rdfs:label "items"@en ;
	rdfs:seeAlso rdf:List ;
	rdfs:seeAlso <https://www.w3.org/TR/activitystreams-vocabulary/#dfn-items> .
#
# http://www.w3.org/ns/activitystreams#last

as:last a owl:ObjectProperty , owl:FunctionalProperty ;
	rdfs:domain as:CollectionPage ;
	rdfs:range as:CollectionPage ;
	rdfs:comment "In a paged Collection, indicates the furthest proceeding page of the collection."@en ;
	rdfs:isDefinedBy <http://www.w3.org/ns/activitystreams> ;
	rdfs:label "last"@en ;
	rdfs:seeAlso as:first , <https://www.w3.org/TR/activitystreams-vocabulary/#dfn-last> .
#
# http://www.w3.org/ns/activitystreams#next

as:next a owl:ObjectProperty , owl:FunctionalProperty ;
	rdfs:domain as:CollectionPage ;
	rdfs:range as:CollectionPage ;
	rdfs:comment "In a paged Collection, indicates the next page of items."@en ;
	rdfs:isDefinedBy <http://www.w3.org/ns/activitystreams> ;
	rdfs:label "next"@en ;
	rdfs:seeAlso as:prev , <https://www.w3.org/TR/activitystreams-vocabulary/#dfn-next> .
#
# http://www.w3.org/ns/activitystreams#partOf

as:partOf a owl:ObjectProperty ;
	rdfs:domain as:CollectionPage ;
	rdfs:range as:Collection ;
	rdfs:comment "Identifies the Collection to which a CollectionPage objects items belong." ;
	rdfs:isDefinedBy <http://www.w3.org/ns/activitystreams> ;
	rdfs:label "partOf"@en ;
	rdfs:seeAlso <https://www.w3.org/TR/activitystreams-vocabulary/#dfn-partof> .
#
# http://www.w3.org/ns/activitystreams#prev

as:prev a owl:ObjectProperty , owl:FunctionalProperty ;
	rdfs:domain as:CollectionPage ;
	rdfs:range as:CollectionPage ;
	rdfs:comment "In a paged Collection, identifies the previous page of items."@en ;
	rdfs:isDefinedBy <http://www.w3.org/ns/activitystreams> ;
	rdfs:label "prev"@en ;
	rdfs:seeAlso as:next , <https://www.w3.org/TR/activitystreams-vocabulary/#dfn-prev> .

#
#
# http://www.w3.org/ns/activitystreams#startIndex

as:startIndex a owl:DatatypeProperty ;
	rdfs:domain as:OrderedCollectionPage ;
	rdfs:range xsd:nonNegativeInteger ;
	rdfs:comment "A non-negative integer value identifying the relative position within the logical view of a strictly ordered collection." ;
	rdfs:isDefinedBy <http://www.w3.org/ns/activitystreams> ;
	rdfs:label "as:startIndex"@en ;
	rdfs:seeAlso <https://www.w3.org/TR/activitystreams-vocabulary/#dfn-startindex> .
#
# http://www.w3.org/ns/activitystreams#totalItems

as:totalItems a owl:DatatypeProperty ;
	rdfs:domain as:Collection ;
	rdfs:range xsd:nonNegativeInteger ;
	rdfs:comment "A non-negative integer specifying the total number of objects contained by the logical view of the collection. This number might not reflect the actual number of items serialized within the Collection object instance."@en ;
	rdfs:isDefinedBy <http://www.w3.org/ns/activitystreams> ;
	rdfs:label "as:totalItems"@en ;
	rdfs:seeAlso <https://www.w3.org/TR/activitystreams-vocabulary/#dfn-totalitems> .


#
# http://www.w3.org/ns/activitystreams#Application

as:Application a owl:Class ;
	rdfs:comment "Describes a software application."@en ;
	rdfs:isDefinedBy <http://www.w3.org/ns/activitystreams> ;
	rdfs:label "as:Application"@en ;
	rdfs:seeAlso <https://www.w3.org/TR/activitystreams-vocabulary/#dfn-application> .
#
# http://www.w3.org/ns/activitystreams#Collection

as:Collection a owl:Class ;
	rdfs:comment """A Collection is a subclass of Object that represents ordered or unordered sets of Object or Link instances.

Refer to the Activity Streams 2.0 Core specification for a complete description of the Collection type."""@en ;
	rdfs:isDefinedBy <http://www.w3.org/ns/activitystreams> ;
	rdfs:label "as:Collection"@en ;
	rdfs:seeAlso <https://www.w3.org/TR/activitystreams-vocabulary/#dfn-collection> .
#
# http://www.w3.org/ns/activitystreams#CollectionPage

as:CollectionPage a owl:Class ;
	rdfs:subClassOf as:Collection ;
	rdfs:comment "Used to represent distinct subsets of items from a Collection. Refer to the Activity Streams 2.0 Core for a complete description of the CollectionPage object."@en ;
	rdfs:isDefinedBy <http://www.w3.org/ns/activitystreams> ;
	rdfs:label "as:CollectionPage"@en ;
	rdfs:seeAlso <https://www.w3.org/TR/activitystreams-vocabulary/#dfn-collectionpage> .
#
# http://www.w3.org/ns/activitystreams#OrderedCollection

as:OrderedCollection a owl:Class ;
	rdfs:subClassOf as:Collection ;
	rdfs:comment "A subclass of Collection in which members of the logical collection are assumed to always be strictly ordered." ;
	rdfs:isDefinedBy <http://www.w3.org/ns/activitystreams> ;
	rdfs:label "as:OrderedCollection"@en ;
	rdfs:seeAlso <https://www.w3.org/TR/activitystreams-vocabulary/#dfn-orderedcollection> .
#
# http://www.w3.org/ns/activitystreams#OrderedCollectionPage

as:OrderedCollectionPage a owl:Class ;
	rdfs:subClassOf as:CollectionPage , as:OrderedCollection ;
	rdfs:comment "Used to represent ordered subsets of items from an OrderedCollection. Refer to the Activity Streams 2.0 Core for a complete description of the OrderedCollectionPage object."@en ;
	rdfs:isDefinedBy <http://www.w3.org/ns/activitystreams> ;
	rdfs:label "as:OrderedCollectionPage"@en ;
	rdfs:seeAlso <https://www.w3.org/TR/activitystreams-vocabulary/#dfn-orderedcollectionpage> .
